%
% Copyright © 2017 Peeter Joot.  All Rights Reserved.
% Licenced as described in the file LICENSE under the root directory of this GIT repository.
%
%{
\input{../latex/blogpost.tex}
\renewcommand{\basename}{potentialMethods.tex}
%\renewcommand{\dirname}{notes/phy1520/}
\renewcommand{\dirname}{notes/ece1228-electromagnetic-theory/}
%\newcommand{\dateintitle}{}
%\newcommand{\keywords}{}

\input{../latex/peeter_prologue_print2.tex}

\usepackage{peeters_layout_exercise}
\usepackage{peeters_braket}
\usepackage{peeters_figures}
\usepackage{siunitx}
%\usepackage{mhchem} % \ce{}
\usepackage{macros_bm} % \bcM
%\usepackage{macros_qed} % \qedmarker
%\usepackage{txfonts} % \ointclockwise

\beginArtNoToc

\generatetitle{A comparision of potential methods}
%\chapter{A comparision of potential methods}
%\label{chap:potentialMethods.tex}

\section{Motivation}

Here is a comparison of potential methods in the time domain for solutions of Maxwell's equations.  Following \citep{balanis2005antenna} Maxwell's equations are extended with magnetic sources and currents, as follows

\input{../ece1229-antenna/MaxwellsStatement.tex}

It will be assumed that the media is isotropic with \( \bcB = \mu \bcH \), and \( \bcD = \epsilon \bcE \).  The impedance of the media will be written as \( \eta = \sqrt{\mu/\epsilon} \), and the group velocity of a wave solution will be written as \( v = 1/\sqrt{\epsilon\mu} \).

\section{Traditional vector algebra}

Potential solutions to \cref{eqn:chapter3Notes:19} follow nicely by considering the electric and magnetic source cases separately, and then building a final solution with superposition.

\subsection{No magnetic sources}

When magnetic sources are omitted, it follows from \cref{eqn:chapter3Notes:80} that there is some \( \bcA \) for which

%\begin{dmath}\label{eqn:potentialMethods:20}
\boxedEquation{eqn:potentialMethods:20}{
\bcB = \spacegrad \cross \bcA,
}
%\end{dmath}

Substitution into Faraday's law \cref{eqn:chapter3Notes:20} gives

\begin{dmath}\label{eqn:potentialMethods:40}
\spacegrad \cross \bcE = - \PD{t}{}\lr{ \spacegrad \cross \bcA },
\end{dmath}

or
\begin{dmath}\label{eqn:potentialMethods:60}
\spacegrad \cross \lr{ \bcE + \PD{t}{ \bcA } } = 0.
\end{dmath}

A gradient representation of this curled quantity, say \( -\spacegrad \phi \), will provide the required zero

%\begin{dmath}\label{eqn:potentialMethods:80}
\boxedEquation{eqn:potentialMethods:80}{
\bcE = -\spacegrad \phi -\PD{t}{ \bcA }.
}
%\end{dmath}

The final two Maxwell equations yield

\begin{dmath}\label{eqn:potentialMethods:100}
\begin{aligned}
-\spacegrad^2 \bcA + \spacegrad \lr{ \spacegrad \cdot \bcA } &= \mu \lr{ \bcJ + \epsilon \PD{t}{} \lr{ -\spacegrad \phi -\PD{t}{ \bcA } } } \\
\spacegrad \cdot \lr{ -\spacegrad \phi -\PD{t}{ \bcA } } &= q_e/\epsilon,
\end{aligned}
\end{dmath}

or
%\begin{dmath}\label{eqn:potentialMethods:120}
\boxedEquation{eqn:potentialMethods:120}{
\begin{aligned}
\spacegrad^2 \bcA - \inv{v^2} \PDSq{t}{ \bcA }
- \spacegrad \lr{
\inv{v^2} \PD{t}{\phi}
+\spacegrad \cdot \bcA
}
&= -\mu \bcJ \\
\spacegrad^2 \phi + \PD{t}{} \lr{ \spacegrad \cdot \bcA } &= -q_e/\epsilon.
\end{aligned}
}
%\end{dmath}

Note that the Lorentz condition \( \PDi{t}{(\phi/v^2)} + \spacegrad \cdot \bcA = 0 \) can be imposed to decouple these, leaving non-homogeneous wave equations for the vector and scalar potentials respectively.

\subsection{No electric sources}

Without electric sources, a curl representation of the electric field can be assumed, satisfing Gauss's law

\boxedEquation{eqn:potentialMethods:140}{
\bcD = - \spacegrad \cross \bcK.
}

Substitution into the Maxwell-Faraday law gives
\begin{dmath}\label{eqn:potentialMethods:160}
\spacegrad \cross \lr{ \bcH + \PD{t}{\bcK} } = 0.
\end{dmath}

This is satisfied with any gradient, say, \( -\spacegrad \phi_m \), providing a potential representation for the magnetic field

%\begin{dmath}\label{eqn:potentialMethods:180}
\boxedEquation{eqn:potentialMethods:180}{
\bcH = -\spacegrad \phi_m - \PD{t}{\bcK}.
}
%\end{dmath}

The remaining Maxwell equations provide the required constraints on the potentials

\begin{subequations}
\label{eqn:potentialMethods:200}
\begin{dmath}\label{eqn:potentialMethods:220}
-\spacegrad^2 \bcK + \spacegrad \lr{ \spacegrad \cdot \bcK } = -\epsilon
\lr{
   -\bcM - \mu \PD{t}{}
   \lr{
      -\spacegrad \phi_m - \PD{t}{\bcK}
   }
}
\end{dmath}
\begin{dmath}\label{eqn:potentialMethods:240}
\spacegrad \cdot
\lr{
-\spacegrad \phi_m - \PD{t}{\bcK}
}
= \inv{\mu} q_m,
\end{dmath}
\end{subequations}

or
%\begin{dmath}\label{eqn:potentialMethods:260}
\boxedEquation{eqn:potentialMethods:260}{
\begin{aligned}
\spacegrad^2 \bcK - \inv{v^2} \PDSq{t}{\bcK} - \spacegrad \lr{ \inv{v^2} \PD{t}{\phi_m} + \spacegrad \cdot \bcK } &= -\epsilon \bcM \\
\spacegrad^2 \phi_m + \PD{t}{}\lr{ \spacegrad \cdot \bcK } &= -\inv{\mu} q_m.
\end{aligned}
}
%\end{dmath}

The general solution to Maxwell's equations is therefore
\begin{dmath}\label{eqn:potentialMethods:280}
\begin{aligned}
\bcE &=
-\spacegrad \phi -\PD{t}{ \bcA }
- \inv{\epsilon} \spacegrad \cross \bcK \\
\bcH &=
\inv{\mu} \spacegrad \cross \bcA
-\spacegrad \phi_m - \PD{t}{\bcK},
\end{aligned}
\end{dmath}

subject to the constraints \cref{eqn:potentialMethods:120} and \cref{eqn:potentialMethods:260}.

\section{Covarient formulation}

The GA formulation of Maxwell's equation is

\begin{dmath}\label{eqn:potentialMethods:300}
\begin{aligned}
\bcF &= \bcE + \eta I \bcH \\
\lr{ \spacegrad + \inv{v} \PD{t}{} } \bcF
&=
%\inv{\epsilon v}
\eta
\lr{ v q_\txte - \bcJ }
+ I \lr{ v q_\txtm - \bcM }.
\end{aligned}
\end{dmath}

This can be converted to covariant form, introducing a four-vector basis \( \setlr{ \gamma_\mu } \), where the spatial basis
\( \setlr{ \Be_k = \gamma_k \gamma_0 } \)
is reexpressed in terms of the Dirac basis \( \setlr{ \gamma_\mu } \).
By multiplying from the left with \( \gamma_0 \) a covariant form of Maxwell's equation is obtained

\begin{dmath}\label{eqn:potentialMethods:320}
\grad \bcF = \eta J - I M,
\end{dmath}

where
\begin{dmath}\label{eqn:potentialMethods:340}
\begin{aligned}
J &= \gamma^\mu J_\mu = ( v q_e, \bcJ ) \\
M &= \gamma^\mu M_\mu = ( v q_m, \bcM ) \\
\grad &= \gamma^\mu \partial_\mu = ( (1/v) \partial_t, \spacegrad ) \\
I &= \gamma_0 \gamma_1 \gamma_2 \gamma_3,
\end{aligned}
\end{dmath}

Here the metric choice is \( \gamma_0^2 = 1 = -\gamma_k^2 \).  Note that in this representation the electromagnetic field \( \bcF = \bcE + \eta I \bcH \) is a bivector, not a multivector as it is explicit (frame dependent) spacetime representation of \cref{eqn:potentialMethods:300}.

A potential representation can be obtained as before by considering electric and magnetic sources in sequence and using superposition to assemble a complete potential.

\subsection{No magnetic sources}

Without magnetic sources, Maxwell's equation splits into vector and trivector terms of the form

\begin{subequations}
\label{eqn:potentialMethods:360}
\begin{dmath}\label{eqn:potentialMethods:380}
\grad \cdot \bcF = \eta J
\end{dmath}
\begin{dmath}\label{eqn:potentialMethods:400}
\grad \wedge \bcF = 0.
\end{dmath}
\end{subequations}

A (spacetime) curl representation of the field will satisfy \cref{eqn:potentialMethods:400} allowing an immediate potential solution

\boxedEquation{eqn:potentialMethods:560}{
\begin{aligned}
&\bcF = \grad \wedge P \\
&\grad^2 P - \grad \lr{ \grad \cdot P } = \eta J.
\end{aligned}
}

This can be put into correspondence with \cref{eqn:potentialMethods:120} by noting that

\begin{dmath}\label{eqn:potentialMethods:460}
\begin{aligned}
\grad^2 &= (\gamma^\mu \partial_\mu) \cdot (\gamma^\nu \partial_\nu)  = \inv{v^2} \partial_{tt} - \spacegrad^2 \\
\gamma_0 P &= \gamma_0 \gamma^\mu P_\mu = P_0 + \Be_k P_k = P_0 + \bcP \\
\gamma_0 \grad &= \gamma_0 \gamma^\mu \partial_\mu = \inv{v} \partial_t + \spacegrad \\
\grad \cdot P &= \partial_\mu P^\mu = \inv{v} \partial_t P_0 - \spacegrad \cdot \bcP,
\end{aligned}
\end{dmath}

so multiplying from the left with \( \gamma_0 \) gives

\begin{dmath}\label{eqn:potentialMethods:480}
\lr{ \inv{v^2} \partial_{tt} - \spacegrad^2 } \lr{ P_0 + \bcP } - \lr{ \inv{v} \partial_t + \spacegrad }\lr{ \inv{v} \partial_t P_0 - \spacegrad \cdot \bcP } = \eta( v q_e - \bcJ ),
\end{dmath}

or

\begin{subequations}
\label{eqn:potentialMethods:500}
\begin{dmath}\label{eqn:potentialMethods:520}
\lr{ \inv{v^2} \partial_{tt} - \spacegrad^2 } \bcP - \spacegrad \lr{ \inv{v} \partial_t P_0 - \spacegrad \cdot \bcP } = -\eta \bcJ
\end{dmath}
\begin{dmath}\label{eqn:potentialMethods:540}
\spacegrad^2 P_0 - \inv{v} \partial_t \lr{ \spacegrad \cdot \bcP } = -q_e/\epsilon.
\end{dmath}
\end{subequations}

So

\begin{dmath}\label{eqn:potentialMethods:580}
\begin{aligned}
P_0 &= \phi \\
-\frac{\BP}{v} &= \BA,
\end{aligned}
\end{dmath}

or
\boxedEquation{eqn:potentialMethods:600}{
P = \gamma_0\lr{ \phi - v \BA }.
}

\subsection{No electric sources}

Without electric sources, Maxwell's equation now splits into

\begin{subequations}
\label{eqn:potentialMethods:620}
\begin{dmath}\label{eqn:potentialMethods:640}
\grad \cdot \bcF = 0
\end{dmath}
\begin{dmath}\label{eqn:potentialMethods:660}
\grad \wedge \bcF = -I M.
\end{dmath}
\end{subequations}

Here the dual of a (spacetime) curl yields a solution

%\begin{dmath}\label{eqn:potentialMethods:680}
\boxedEquation{eqn:potentialMethods:680}{
\bcF = I ( \grad \wedge Q ).
}
%\end{dmath}

Substituting this gives

\begin{subequations}
\label{eqn:potentialMethods:700}
\begin{dmath}\label{eqn:potentialMethods:720}
0
=
\grad \cdot (I ( \grad \wedge Q ) )
=
\gpgradeone{ \grad I ( \grad \wedge Q ) }
=
-I \grad \wedge ( \grad \wedge Q ).
\end{dmath}
\begin{dmath}\label{eqn:potentialMethods:740}
-I M
=
\grad \wedge (I ( \grad \wedge Q ) )
=
\gpgradethree{ \grad I ( \grad \wedge Q ) }
=
-I \grad \cdot ( \grad \wedge Q ).
\end{dmath}
\end{subequations}

The \( \grad \cdot \bcF \) relation \cref{eqn:potentialMethods:720} is identically zero as desired, leaving

%\begin{dmath}\label{eqn:potentialMethods:760}
\boxedEquation{eqn:potentialMethods:760}{
\grad^2 Q - \grad \lr{ \grad \cdot Q }
=
M.
}
%\end{dmath}

So the general solution with both electric and magnetic sources is

%\begin{dmath}\label{eqn:potentialMethods:800}
\boxedEquation{eqn:potentialMethods:800}{
\bcF = \grad \wedge P + I (\grad \wedge Q),
}
%\end{dmath}

subject to the constraints of \cref{eqn:potentialMethods:560} and \cref{eqn:potentialMethods:760}.  As before the four-potential \( Q \) can be put into correspondance with the conventional scalar and vector potentials by left multiplying with \( \gamma_0 \), which gives

\begin{dmath}\label{eqn:potentialMethods:820}
\lr{ \inv{v^2} \partial_{tt} - \spacegrad^2 } \lr{ Q_0 + \bcQ } - \lr{ \inv{v} \partial_t + \spacegrad }\lr{ \inv{v} \partial_t Q_0 - \spacegrad \cdot \bcQ } = v q_m - \bcM,
\end{dmath}

or
\begin{subequations}
\label{eqn:potentialMethods:840}
\begin{dmath}\label{eqn:potentialMethods:860}
\lr{ \inv{v^2} \partial_{tt} - \spacegrad^2 } \bcQ - \spacegrad \lr{ \inv{v} \partial_t Q_0 - \spacegrad \cdot \bcQ } = - \bcM
\end{dmath}
\begin{dmath}\label{eqn:potentialMethods:880}
\spacegrad^2 Q_0 - \inv{v} \partial_t \spacegrad \cdot \bcQ = -v q_m.
\end{dmath}
\end{subequations}

Comparing with \cref{eqn:potentialMethods:260} shows that

\boxedEquation{eqn:potentialMethods:260}{
\begin{aligned}
\spacegrad^2 \bcK - \inv{v^2} \PDSq{t}{\bcK} - \spacegrad \lr{ \inv{v^2} \PD{t}{\phi_m} + \spacegrad \cdot \bcK } &= -\epsilon \bcM \\
\spacegrad^2 \phi_m + \PD{t}{}\lr{ \spacegrad \cdot \bcK } &= -\inv{\mu} q_m.
\end{aligned}
}
%\end{dmath}

%}
\EndArticle
